[coq] Type-safety of STLC via logical relations

coq/simple-types/SemanticsSOS.v
@@ -2,6 +2,7 @@
 
 Require Import Utf8.
 Require Import Syntax.
+Require Import Relation_Operators.
 
 (** SOS reduction rules *)
 Inductive red {A : Set} : expr A → expr A → Prop :=
@@ -16,3 +17,107 @@ Inductive red {A : Set} : expr A → expr A → Prop :=
     red e e' →
     red (e_app v e) (e_app v e')
 .
+
+(** Reflexive and transitive closure of a reduction relation *)
+Notation red_rtc e₁ e₂ := (clos_refl_trans_1n _ red e₁ e₂).
+
+Inductive is_value {A : Set} : expr A → Prop :=
+| is_val : ∀ v : value _, is_value v
+.
+
+Lemma is_value_dec {A : Set} (e : expr A) :
+  {is_value e} + {¬is_value e}.
+Proof.
+  destruct e;
+    (left; constructor; fail) ||
+    (right; intro H; inversion H).
+Qed.
+
+(** Safety property *)
+Definition safe {A : Set} (e : expr A) : Prop :=
+  ∀ e', red_rtc e e' → is_value e' ∨ ∃ e'', red e' e''.
+
+(** Reduction is deterministic *)
+Lemma red_deterministic {A : Set} {e e₁ e₂ : expr A} :
+  red e e₁ → red e e₂ → e₁ = e₂.
+Proof.
+  intro Hred; generalize e₂; clear e₂.
+  induction Hred; intros ? Hred2; inversion Hred2; subst; clear Hred2;
+    repeat match goal with
+    | [ |- ?e = ?e ] => reflexivity
+    | [ H: red (e_value _) _ |- _ ] => inversion H (* values do not reduce *)
+    | [ IH: ∀ _, red _ _ → _ = _ |- _ ] =>
+      erewrite IH; [ reflexivity | ]; assumption
+    end.
+Qed.
+
+Lemma red_rtc_app1 {A : Set} (e₁ e₁' e₂ : expr A) :
+  red_rtc e₁ e₁' →
+  red_rtc (e_app e₁ e₂) (e_app e₁' e₂).
+Proof.
+  induction 1; econstructor; [ apply red_app1 | ]; eassumption.
+Qed.
+
+Lemma value_red_rtc_to_value {A : Set} (v : value A) e :
+  red_rtc v e → is_value e.
+Proof.
+  inversion 1; [ constructor | ].
+  match goal with
+  | [ H: red (e_value _) _ |- _ ] => inversion H
+  end.
+Qed.
+
+(* ========================================================================= *)
+(* Inversion of reflexive-transitive closure of reduction for application.
+ * During the lecture, we said that the main lemma of this section
+ * `red_rtc_app_inv` is obvious. In Coq we have to prove it, and it requires
+ * some work. These lemma is important only in the SafetyLogicalRealtion. *)
+
+Inductive red_rtc_app_inv_class {A : Set} (e₁ e₂ : expr A) : expr A → Prop :=
+| rrapp_inv1 : ∀ e₁',
+    red_rtc e₁ e₁' →
+    ¬ is_value e₁' →
+    red_rtc_app_inv_class e₁ e₂ (e_app e₁' e₂)
+| rrapp_inv2 : ∀ (v₁ : value A) e₂',
+    red_rtc e₁ v₁ →
+    red_rtc e₂ e₂' →
+    ¬ is_value e₂' →
+    red_rtc_app_inv_class e₁ e₂ (e_app v₁ e₂')
+| rrapp_inv3 : ∀ (v₁ v₂ : value A) e,
+    red_rtc e₁ v₁ →
+    red_rtc e₂ v₂ →
+    red_rtc (e_app v₁ v₂) e →
+    red_rtc_app_inv_class e₁ e₂ e
+.
+
+Lemma red_rtc_app_inv {A : Set} {e₁ e₂ e : expr A} :
+  red_rtc (e_app e₁ e₂) e → red_rtc_app_inv_class e₁ e₂ e.
+Proof.
+  intro Hred; remember (e_app e₁ e₂) as e₀.
+  generalize e₁ e₂ Heqe₀; clear e₁ e₂ Heqe₀.
+  induction Hred as [ | e e' e'' Hred Hrtc IH ].
+  + intros e₁ e₂ Heq; subst.
+    destruct (is_value_dec e₁) as [ [ v₁ ] | ].
+    - destruct (is_value_dec e₂) as [ [ v₂ ] | ].
+      * eapply rrapp_inv3; constructor.
+      * apply rrapp_inv2; try assumption; constructor.
+    - apply rrapp_inv1; [ constructor | assumption ].
+  + intros e₁ e₂ Heq; subst.
+    inversion Hred; clear Hred; subst.
+    - eapply rrapp_inv3; [ constructor | constructor | ].
+      econstructor; [ apply red_beta | eassumption ].
+    - specialize (IH _ _ eq_refl); destruct IH.
+      * apply rrapp_inv1; [ | assumption ].
+        econstructor; eassumption.
+      * apply rrapp_inv2; try assumption; [].
+        econstructor; eassumption.
+      * eapply rrapp_inv3; try eassumption; [].
+        econstructor; eassumption.
+    - specialize (IH _ _ eq_refl); destruct IH as [ ? ? Hval | | ].
+      * exfalso; apply Hval.
+        eapply value_red_rtc_to_value; eassumption.
+      * apply rrapp_inv2; try assumption; [].
+        econstructor; eassumption.
+      * eapply rrapp_inv3; try eassumption; [].
+        econstructor; eassumption.
+Qed.
