coq/simple-types/SafetyLogicalRelation.v
@@ -1,0 +1,178 @@
+(** Here, we prove type-soundness using logical relations. *)
+
+Require Import Utf8.
+Require Import Syntax SemanticsSOS Typing.
+
+(** Semantic types: unary relations on closed values *)
+Definition SemType : Type := value Empty_set → Prop.
+
+(** Expression closure of a semantic type *)
+Definition EClo (R : SemType) (e : expr Empty_set) :=
+  ∀ e', red_rtc e e' →
+    (∃ v : value _, R v ∧ e' = v) ∨
+    (∃ e'', red e' e'').
+
+(** Relation EClo R contains values of a semantic type R *)
+Lemma EClo_value (R : SemType) v :
+  R v → EClo R v.
+Proof.
+  intros Hv e; destruct 1 as [ | ? ? Hred ].
+  + left; eauto.
+  + (* impossible case: values don't reduce *)
+    inversion Hred.
+Qed.
+
+(** EClo is preserved by a backward reduction *)
+Lemma EClo_red (R : SemType) e e' :
+  red e e' → EClo R e' → EClo R e.
+Proof.
+  intros Hred He' e₁ He₁.
+  destruct He₁ as [ | e₂ e₃ Hred₁ ].
+  + right; eauto.
+  + apply He'.
+    rewrite (red_deterministic Hred Hred₁); assumption.
+Qed.
+
+(* ========================================================================= *)
+(* Denotation of types *)
+
+Reserved Notation "'⟦' τ '⟧'".
+
+(* For convenience, for each type construct we define a corresponding
+ * operation on semantic types *)
+
+(** Semantic Unit type. Because we require a concrete shape of a value, it
+  * is convenient to define this relation as an inductive type. *)
+Inductive Rel_Unit : SemType :=
+| RU_unit : Rel_Unit v_unit
+.
+
+(** Semantic Arrow type *)
+Definition Rel_Arrow (R₁ R₂ : SemType) : SemType :=
+  λ v, ∀ v', R₁ v' → EClo R₂ (e_app v v').
+
+(** Denotation of types *)
+Fixpoint relT (τ : type) : SemType :=
+  match τ with
+  | t_unit        => Rel_Unit
+  | t_arrow τ₁ τ₂ => Rel_Arrow ⟦ τ₁ ⟧ ⟦ τ₂ ⟧
+  end
+where "⟦ τ ⟧" := (relT τ).
+
+(** Denotation of typing environments *)
+Definition rel_g {A : Set} (Γ : env A) (γ : A → value _) : Prop :=
+  ∀ x, ⟦ Γ x ⟧ (γ x).
+
+Notation "'G⟦' Γ '⟧'" := (@rel_g _ Γ).
+
+(** The logical relation *)
+Definition rel_e {A : Set} (Γ : env A) (e : expr A) (τ : type) : Prop :=
+  ∀ γ, G⟦ Γ ⟧ γ → EClo ⟦ τ ⟧ (ebind γ e).
+
+Notation "'T⟦' Γ '⊨' e '∷' τ '⟧'" := (@rel_e _ Γ e τ).
+
+Lemma rel_g_env_ext {A : Set} (Γ : env A) (τ : type) γ v :
+  G⟦ Γ ⟧ γ → ⟦ τ ⟧ v → G⟦ env_ext Γ τ ⟧ (scons v γ).
+Proof.
+  intros Hγ Hτ [ | x ]; simpl; [ assumption | apply Hγ ].
+Qed.
+
+(* ========================================================================= *)
+(* Compatibility lemmas *)
+
+Lemma compat_unit {A : Set} (Γ : env A) :
+  T⟦ Γ ⊨ v_unit ∷ t_unit ⟧.
+Proof.
+  intros γ Hγ.
+  apply EClo_value; constructor.
+Qed.
+
+Lemma compat_var {A : Set} (Γ : env A) x :
+  T⟦ Γ ⊨ v_var x ∷ Γ x ⟧.
+Proof.
+  intros γ Hγ.
+  apply EClo_value, Hγ.
+Qed.
+
+Lemma compat_lam {A : Set} (Γ : env A) e τ₁ τ₂ :
+  T⟦ env_ext Γ τ₁ ⊨ e ∷ τ₂ ⟧ →
+  T⟦ Γ ⊨ v_lam e ∷ t_arrow τ₁ τ₂ ⟧.
+Proof.
+  intros He γ Hγ; simpl.
+  apply EClo_value.
+  intros v Hv.
+  eapply EClo_red; [ apply red_beta | ].
+  rewrite esubst_bind_lift. (* we merge two substitutions *)
+  apply He.
+  apply rel_g_env_ext; assumption.
+Qed.
+
+(** Closed version of application copatibility *)
+Lemma compat_app_cl e₁ e₂ (R₂ R₁ : SemType) :
+  EClo (Rel_Arrow R₂ R₁) e₁ →
+  EClo R₂ e₂ →
+  EClo R₁ (e_app e₁ e₂).
+Proof.
+  intros He₁ He₂ e Hred.
+  destruct (red_rtc_app_inv Hred) as [ e₁' ? Hval | v₁ e₂' ? ? Hval | v₁ v₂ ].
+  + right; specialize (He₁ e₁').
+    destruct He₁ as [ [ v [ _ ? ] ] | [ e₁'' Hred₁ ] ];
+      [ assumption | subst; exfalso; apply Hval; constructor | ].
+    eexists; apply red_app1; eassumption.
+  + right; specialize (He₂ e₂').
+    destruct He₂ as [ [ v [ _ ? ] ] | [ e₂'' Hred₂ ] ];
+      [ assumption | subst; exfalso; apply Hval; constructor | ].
+    eexists; apply red_app2; eassumption.
+  + specialize (He₁ v₁).
+    destruct He₁ as [ [ v₁' [ Hv₁ Heq ] ] | [ ? Hred₁ ] ];
+      [ assumption | | inversion Hred₁ ].
+    injection Heq; clear Heq; intro; subst.
+    specialize (He₂ v₂).
+    destruct He₂ as [ [ v₂' [ Hv₂ Heq ] ] | [ ? Hred₂ ] ];
+      [ assumption | | inversion Hred₂ ].
+    injection Heq; clear Heq; intro; subst.
+    eapply Hv₁; eassumption.
+Qed.
+
+Lemma compat_app {A : Set} (Γ : env A) e₁ e₂ τ₂ τ₁ :
+  T⟦ Γ ⊨ e₁ ∷ t_arrow τ₂ τ₁ ⟧ →
+  T⟦ Γ ⊨ e₂ ∷ τ₂ ⟧ →
+  T⟦ Γ ⊨ e_app e₁ e₂ ∷ τ₁ ⟧.
+Proof.
+  intros He₁ He₂ γ Hγ; simpl.
+  eapply compat_app_cl; [ eapply He₁ | eapply He₂ ]; assumption.
+Qed.
+
+(* ========================================================================= *)
+(* Soundness *)
+
+Theorem fundamental_property {A : Set} (Γ : env A) e τ :
+  T[ Γ ⊢ e ∷ τ ] → T⟦ Γ ⊨ e ∷ τ ⟧.
+Proof.
+  induction 1.
+  + apply compat_unit.
+  + apply compat_var.
+  + apply compat_lam; assumption.
+  + eapply compat_app; eassumption.
+Qed.
+
+Theorem adequacy (R : SemType) e :
+  EClo R e → safe e.
+Proof.
+  intros He e' Hred; specialize (He e' Hred).
+  destruct He as [ [ v [ _ Heq ] ] | [ e'' Hred' ] ].
+  + left; subst; constructor.
+  + right; eauto.
+Qed.
+
+Theorem type_safety e τ :
+  T[ env_empty ⊢ e ∷ τ ] → safe e.
+Proof.
+  (* This is one of these rare cases where forward reasoning is more
+   * convenient. *)
+  intro He; apply fundamental_property in He.
+  specialize (He v_var).
+  rewrite ebind_pure' in He.
+  eapply adequacy, He.
+  intros [].
+Qed.
